__________________________________________________________________________
#### **Tags:** #Math/SetTheory 
###### *Date of Creation: 2023-09-24*
__________________________________________________________________________

Inverse of h o f = identity function of x
Inverse of f o h = identity function of y

Taking the inverse of a composite function, ex. (g o f)^-1, you must swap the order of the functions, ex. f^-1 o g^-1

Lemma: If h and k are both inverses of f, h: Y -> X, k: Y -> X and f: X -> Y. then h = k

Proof: To show that for all y e Y  h(y) = k(y). Shortcut: use properties of inverse.

h = h o identity of y = h o (f o k) = (h o f) o k = identity of x o k = k

thus h is equal to k. 
#### Sources:
__________________________________________________________________________
1. 